\textit{Response.}

Consider the following SDE

\begin{equation}
	dx = -a\,x\,dt + t\,dW,
\end{equation}

where $x$ is real and $a >0$ is constant. The mean of $x$ changes according to

\begin{equation}
	d\gang{x} = -a\,\gang{x}\,dt,
\end{equation}

which we may solve analytically

\begin{equation}
	\gang{x} = \gang{x_0}\,e^{-a\,t}
\end{equation}

where $\gang{x_0}$ is the mean of the initial distribution of $x$. As $t \to \infty$, $\gang{x}$ decays to zero from any initial value.

To calculate the variance, we first write the evolution of $x' = x - \gang{x}$

\begin{equation}
	dx' = -a\,x'\,dt + t\,dW,
\end{equation}

Using It\^{o}'s formula, we have

\begin{align}
	d\vr{x} &= d\gang{\gpr{x'}^2} = \gang{2\,x'\,dx'} + \gang{\gpr{dx'}^2} \nonumber \\
		&= \gpr{-2\,a\,\gang{\gpr{x'}^2} + t^2}\,dt.
\end{align}

whose solution may be written explicitly

\begin{equation}
	\vr{x} = \gpr{\vr{x_0} - \frac{1}{4\,a^3}}\,e^{-2\,a\,t} + \frac{1 - 2\,a\,t + 2\,a^2\,t^2}{4\,a^3}.
\end{equation}

We may readily see that as $t \to \infty$, the variance goes like $t^2$ which is unbounded.

