\textit{Response.}

We begin by writing the most general form of a linear stochastic differential equation with multiplicative noise

\begin{equation}
	d \func{x}{t} = -\lambda\,\gpr{\func{x}{t} - \mu}\,dt + \func{\sigma}{t,\ \func{x}{t}}\,d \func{W}{t},
\end{equation}

where $\lambda > 0$ is real, and $\mu$ is the mean of the target distribution. For our case, $\mu = 1$.

The Fokker-Planck equation gives a differential equation for the equilibrium distribution

\begin{equation}
	-\partial_{x} \gbkt{-\lambda\,\gpr{x - \mu}\,\func{p}{x}} + \frac{1}{2}\,\partial_x^2 \gbkt{\gpr{\func{\sigma}{x}}^2\,\func{p}{x}} = 0,
\end{equation}

where we have simply set $\partial_t p = 0$ in the time-dependent Fokker-Planck equation. We may integrate both sides of this equation to obtain

\begin{equation}
	\lambda\,\gpr{x - \mu}\,\func{p}{x} + \frac{1}{2}\,\partial_x \gbkt{\gpr{\func{\sigma}{x}}^2\,\func{p}{x}} = \mathcal{C}_1,
\end{equation}

where $\mathcal{C}_1$ is a constant of integration. Pugging in the desired distribution to the first term on the left-hand side and rearranging, we obtain

\begin{equation}
	\partial_x \gbkt{\gpr{\func{\sigma}{x}}^2\,\func{p}{x}} = 2\,\gpr{\mathcal{C}_1 - \lambda\,\alpha\,\gpr{x - \mu}\,x^{-\gpr{\alpha + 1}}}.
\end{equation}

We can integrate this equation once more to obtain

\begin{equation}
	\gpr{\func{\sigma}{x}}^2\,\func{p}{x} = 2\,\gpr{\mathcal{C}_1\,x + \frac{1}{2}\,\mathcal{C}_2 - \lambda\,\gpr{\frac{\alpha}{1 - \alpha}\,x^{1-\alpha} - \mu\,x^{-\alpha}}}.
\end{equation}

In the limit as $x \to \infty$, the left-hand side decays to zero, and so the right-hand side must decay to zero as well, i.e., $\mathcal{C}_1 = \mathcal{C}_2 = 0$. Therefore,

\begin{equation}
	\gpr{\func{\sigma}{x}}^2 = 2\,\lambda\,x\,\gpr{\frac{\mu}{\alpha} - \frac{1}{1 - \alpha}\,x}.
\end{equation}

Taking $\func{\sigma}{x}$ to be non-negative, we obtain the the desired one-dimensional linear stochastic differential equation

\begin{equation}
	d\func{x}{t} = -\lambda\,\gpr{\func{x}{t} - 1}\,dt + \sqrt{2\,\lambda\,\func{x}{t}\,\gpr{\frac{1}{\alpha} - \frac{1}{1 - \alpha}\,\func{x}{t}}}\,d \func{W}{t}.
\end{equation}

Note that the term under the square root is positive for $\frac{1 - \alpha}{\alpha} < \func{x}{t}$, which is always true given the conditions on $\alpha$ and $\func{x}{t}$.

